guard pages WIP: src/SlabsAlloc WIP

src/SlabsAlloc.fst
@@ -437,8 +437,6 @@ let allocate_slab_aux_1
 
 #restart-solver
 
-//checkpoint
-
 inline_for_extraction noextract
 let allocate_slab_aux_2_full
   (size_class: sc)
@@ -446,21 +444,22 @@ let allocate_slab_aux_2_full
   (md_bm_region: array U64.t{A.length md_bm_region = U32.v metadata_max * 4})
   (md_region: array AL.cell{A.length md_region = U32.v metadata_max})
   (md_count: ref U32.t)
-  (r1 r2 r3: ref US.t)
+  (r1 r2 r3 r4: ref US.t)
   (md_count_v: U32.t{U32.v md_count_v <= U32.v metadata_max})
   (md_region_lv: G.erased (Seq.lseq AL.status (U32.v md_count_v)))
   (idx1: US.t)
   (idx2: US.t{US.v idx2 < U32.v md_count_v})
-  (idx3: US.t)
+  (idx3 idx4: US.t)
   : Steel unit
   (
     vptr md_count `star`
     vptr r1 `star`
     vptr r2 `star`
     vptr r3 `star`
-    (AL.varraylist pred1 pred2 pred3
+    vptr r4 `star`
+    (AL.varraylist pred1 pred2 pred3 pred4
       (A.split_l md_region (u32_to_sz md_count_v))
-      (US.v idx1) (US.v idx2) (US.v idx3)) `star`
+      (US.v idx1) (US.v idx2) (US.v idx3) (US.v idx4)) `star`
     starseq
       #(pos:U32.t{U32.v pos < U32.v md_count_v})
       #(t size_class)
@@ -472,50 +471,55 @@ let allocate_slab_aux_2_full
     vrefinedep
       (vptr md_count)
       vrefinedep_prop
-      (left_vprop size_class slab_region md_bm_region md_region r1 r2 r3)
+      (left_vprop size_class slab_region md_bm_region md_region r1 r2 r3 r4)
   )
   (requires fun h0 ->
-    let gs0 = AL.v_arraylist pred1 pred2 pred3 (A.split_l md_region (u32_to_sz md_count_v)) (US.v idx1) (US.v idx2) (US.v idx3) h0 in
+    let gs0 = AL.v_arraylist pred1 pred2 pred3 pred4
+      (A.split_l md_region (u32_to_sz md_count_v))
+      (US.v idx1) (US.v idx2) (US.v idx3) (US.v idx4) h0 in
     U32.v md_count_v <> AL.null /\
     sel md_count h0 == md_count_v /\
     sel r1 h0 == idx1 /\
     sel r2 h0 == idx2 /\
     sel r3 h0 == idx3 /\
+    sel r4 h0 == idx4 /\
     idx2 <> AL.null_ptr /\
     ALG.dataify gs0 `Seq.equal` G.reveal md_region_lv /\
-    ALG.partition #AL.status gs0 (US.v idx1) (US.v idx2) (US.v idx3)
+    ALG.partition #AL.status gs0 (US.v idx1) (US.v idx2) (US.v idx3) (US.v idx4)
   )
   (ensures fun _ _ h1 ->
     let blob1
       = h1 (vrefinedep
       (vptr md_count)
       vrefinedep_prop
-      (left_vprop size_class slab_region md_bm_region md_region r1 r2 r3)
+      (left_vprop size_class slab_region md_bm_region md_region r1 r2 r3 r4)
     ) in
     md_count_v == dfst blob1)
   =
-  (**) let gs0 = gget (AL.varraylist pred1 pred2 pred3 (A.split_l md_region (u32_to_sz md_count_v)) (US.v idx1) (US.v idx2) (US.v idx3)) in
-  (**) ALG.lemma_head_not_null_mem pred1 pred2 pred3
+  (**) let gs0 = gget (AL.varraylist pred1 pred2 pred3 pred4
     (A.split_l md_region (u32_to_sz md_count_v))
-    idx1 idx2 idx3;
-  let idx2' = AL.remove2 #pred1 #pred2 #pred3
+    (US.v idx1) (US.v idx2) (US.v idx3) (US.v idx4)) in
+  (**) ALG.lemma_head_not_null_mem pred1 pred2 pred3 pred4
     (A.split_l md_region (u32_to_sz md_count_v))
-    (Ghost.hide (US.v idx1)) idx2 (Ghost.hide (US.v idx3)) idx2 in
+    idx1 idx2 idx3 idx4;
+  let idx2' = AL.remove2 #pred1 #pred2 #pred3 #pred4
+    (A.split_l md_region (u32_to_sz md_count_v))
+    (G.hide (US.v idx1)) idx2 (G.hide (US.v idx3)) (G.hide (US.v idx4)) idx2 in
   AL.insert3 #pred1 #pred2 #pred3
     (A.split_l md_region (u32_to_sz md_count_v))
-    idx3 (Ghost.hide (US.v idx1)) (Ghost.hide (US.v idx2')) idx2 2ul;
+    idx3 (G.hide (US.v idx1)) (G.hide (US.v idx2')) (G.hide (US.v idx4)) idx2 2ul;
   write r2 idx2';
   write r3 idx2;
 
-  (**) let gs1 = gget (AL.varraylist pred1 pred2 pred3
+  (**) let gs1 = gget (AL.varraylist pred1 pred2 pred3 pred4
     (A.split_l md_region (u32_to_sz md_count_v))
-    (US.v idx1) (US.v idx2') (US.v idx2)) in
-  assert (ALG.ptrs_all #AL.status (US.v idx1) (US.v idx2) (US.v idx3) gs0 `FStar.FiniteSet.Base.equal`
-          ALG.ptrs_all #AL.status (US.v idx1) (US.v idx2') (US.v idx2) gs1);
+    (US.v idx1) (US.v idx2') (US.v idx2) (US.v idx4)) in
+  assert (ALG.ptrs_all #AL.status (US.v idx1) (US.v idx2) (US.v idx3) (US.v idx4) gs0 `FStar.FiniteSet.Base.equal`
+          ALG.ptrs_all #AL.status (US.v idx1) (US.v idx2') (US.v idx2) (US.v idx4) gs1);
 
-  (**) pack_3 size_class slab_region md_bm_region md_region md_count r1 r2 r3
+  (**) pack_3 size_class slab_region md_bm_region md_region md_count r1 r2 r3 r4
     md_count_v (G.hide (Seq.upd (G.reveal md_region_lv) (US.v idx2) 2ul))
-    idx1 idx2' idx2
+    idx1 idx2' idx2 idx4
 
 inline_for_extraction noextract
 let allocate_slab_aux_2_partial
@@ -524,21 +528,22 @@ let allocate_slab_aux_2_partial
   (md_bm_region: array U64.t{A.length md_bm_region = U32.v metadata_max * 4})
   (md_region: array AL.cell{A.length md_region = U32.v metadata_max})
   (md_count: ref U32.t)
-  (r1 r2 r3: ref US.t)
+  (r1 r2 r3 r4: ref US.t)
   (md_count_v: U32.t{U32.v md_count_v <= U32.v metadata_max})
   (md_region_lv: G.erased (Seq.lseq AL.status (U32.v md_count_v)))
   (idx1: US.t)
   (idx2: US.t{US.v idx2 < U32.v md_count_v})
-  (idx3: US.t)
+  (idx3 idx4: US.t)
   : Steel unit
   (
     vptr md_count `star`
     vptr r1 `star`
     vptr r2 `star`
     vptr r3 `star`
-    (AL.varraylist pred1 pred2 pred3
+    vptr r4 `star`
+    (AL.varraylist pred1 pred2 pred3 pred4
       (A.split_l md_region (u32_to_sz md_count_v))
-      (US.v idx1) (US.v idx2) (US.v idx3)) `star`
+      (US.v idx1) (US.v idx2) (US.v idx3) (US.v idx4)) `star`
     starseq
       #(pos:U32.t{U32.v pos < U32.v md_count_v})
       #(t size_class)
@@ -550,31 +555,34 @@ let allocate_slab_aux_2_partial
     vrefinedep
       (vptr md_count)
       vrefinedep_prop
-      (left_vprop size_class slab_region md_bm_region md_region r1 r2 r3)
+      (left_vprop size_class slab_region md_bm_region md_region r1 r2 r3 r4)
   )
   (requires fun h0 ->
-    let gs0 = AL.v_arraylist pred1 pred2 pred3 (A.split_l md_region (u32_to_sz md_count_v)) (US.v idx1) (US.v idx2) (US.v idx3) h0 in
+    let gs0 = AL.v_arraylist pred1 pred2 pred3 pred4
+      (A.split_l md_region (u32_to_sz md_count_v))
+      (US.v idx1) (US.v idx2) (US.v idx3) (US.v idx4) h0 in
     U32.v md_count_v <> AL.null /\
     sel md_count h0 == md_count_v /\
     sel r1 h0 == idx1 /\
     sel r2 h0 == idx2 /\
     sel r3 h0 == idx3 /\
+    sel r4 h0 == idx4 /\
     idx2 <> AL.null_ptr /\
     ALG.dataify gs0 `Seq.equal` G.reveal md_region_lv /\
-    ALG.partition #AL.status gs0 (US.v idx1) (US.v idx2) (US.v idx3)
+    ALG.partition #AL.status gs0 (US.v idx1) (US.v idx2) (US.v idx3) (US.v idx4)
   )
   (ensures fun _ _ h1 ->
     let blob1
       = h1 (vrefinedep
       (vptr md_count)
       vrefinedep_prop
-      (left_vprop size_class slab_region md_bm_region md_region r1 r2 r3)
+      (left_vprop size_class slab_region md_bm_region md_region r1 r2 r3 r4)
     ) in
     md_count_v == dfst blob1)
   =
-  (**) pack_3 size_class slab_region md_bm_region md_region md_count r1 r2 r3
+  (**) pack_3 size_class slab_region md_bm_region md_region md_count r1 r2 r3 r4
     md_count_v md_region_lv
-    idx1 idx2 idx3
+    idx1 idx2 idx3 idx4
 
 inline_for_extraction noextract
 let allocate_slab_aux_2
@@ -583,19 +591,20 @@ let allocate_slab_aux_2
   (md_bm_region: array U64.t{A.length md_bm_region = U32.v metadata_max * 4})
   (md_region: array AL.cell{A.length md_region = U32.v metadata_max})
   (md_count: ref U32.t)
-  (r1 r2 r3: ref US.t)
+  (r1 r2 r3 r4: ref US.t)
   (md_count_v: U32.t{U32.v md_count_v <= U32.v metadata_max})
   (md_region_lv: G.erased (Seq.lseq AL.status (U32.v md_count_v)))
-  (idx1 idx2 idx3: US.t)
+  (idx1 idx2 idx3 idx4: US.t)
   : Steel (array U8.t)
   (
     vptr md_count `star`
     vptr r1 `star`
     vptr r2 `star`
     vptr r3 `star`
-    (AL.varraylist pred1 pred2 pred3
+    vptr r4 `star`
+    (AL.varraylist pred1 pred2 pred3 pred4
       (A.split_l md_region (u32_to_sz md_count_v))
-      (US.v idx1) (US.v idx2) (US.v idx3)) `star`
+      (US.v idx1) (US.v idx2) (US.v idx3) (US.v idx4)) `star`
     starseq
       #(pos:U32.t{U32.v pos < U32.v md_count_v})
       #(t size_class)
@@ -608,31 +617,34 @@ let allocate_slab_aux_2
     vrefinedep
       (vptr md_count)
       vrefinedep_prop
-      (left_vprop size_class slab_region md_bm_region md_region r1 r2 r3)
+      (left_vprop size_class slab_region md_bm_region md_region r1 r2 r3 r4)
   )
   (requires fun h0 ->
-    let gs0 = AL.v_arraylist pred1 pred2 pred3 (A.split_l md_region (u32_to_sz md_count_v)) (US.v idx1) (US.v idx2) (US.v idx3) h0 in
+    let gs0 = AL.v_arraylist pred1 pred2 pred3 pred4
+      (A.split_l md_region (u32_to_sz md_count_v))
+      (US.v idx1) (US.v idx2) (US.v idx3) (US.v idx4) h0 in
     U32.v md_count_v <> AL.null /\
     sel md_count h0 == md_count_v /\
     sel r1 h0 == idx1 /\
     sel r2 h0 == idx2 /\
     sel r3 h0 == idx3 /\
+    sel r4 h0 == idx4 /\
     idx2 <> AL.null_ptr /\
     ALG.dataify gs0 `Seq.equal` G.reveal md_region_lv /\
-    ALG.partition #AL.status gs0 (US.v idx1) (US.v idx2) (US.v idx3)
+    ALG.partition #AL.status gs0 (US.v idx1) (US.v idx2) (US.v idx3) (US.v idx4)
   )
   (ensures fun _ _ h1 ->
     let blob1
       = h1 (vrefinedep
       (vptr md_count)
       vrefinedep_prop
-      (left_vprop size_class slab_region md_bm_region md_region r1 r2 r3)
+      (left_vprop size_class slab_region md_bm_region md_region r1 r2 r3 r4)
     ) in
     md_count_v == dfst blob1)
   =
-  (**) ALG.lemma_head2_in_bounds pred1 pred2 pred3
+  (**) ALG.lemma_head2_in_bounds pred1 pred2 pred3 pred4
     (A.split_l md_region (u32_to_sz md_count_v))
-    (US.v idx1) idx2 (US.v idx3);
+    (US.v idx1) idx2 (US.v idx3) (US.v idx4);
   (**) starseq_unpack_s
     #_
     #(pos:U32.t{U32.v pos < U32.v md_count_v})
@@ -642,11 +654,13 @@ let allocate_slab_aux_2
     (SeqUtils.init_u32_refined (U32.v md_count_v))
     (US.v idx2);
 
-  (**) ALG.lemma_head2_implies_pred2 pred1 pred2 pred3 (A.split_l md_region (u32_to_sz md_count_v)) idx1 idx2 idx3;
+  (**) ALG.lemma_head2_implies_pred2 pred1 pred2 pred3 pred4
+    (A.split_l md_region (u32_to_sz md_count_v))
+    idx1 idx2 idx3 idx4;
 
-  (**) let gs0 = gget (AL.varraylist pred1 pred2 pred3
-                                (A.split_l md_region (u32_to_sz md_count_v))
-                                (US.v idx1) (US.v idx2) (US.v idx3)) in
+  (**) let gs0 = gget (AL.varraylist pred1 pred2 pred3 pred4
+    (A.split_l md_region (u32_to_sz md_count_v))
+    (US.v idx1) (US.v idx2) (US.v idx3) (US.v idx4)) in
 
   (**) ALG.lemma_dataify_index #AL.status gs0 (US.v idx2);
   (**) SeqUtils.init_u32_refined_index (U32.v md_count_v) (US.v idx2);
@@ -667,15 +681,15 @@ let allocate_slab_aux_2
   in
   if cond then (
     (**) pack_slab_starseq size_class
-      slab_region md_bm_region md_region md_count r1 r2 r3
+      slab_region md_bm_region md_region md_count r1 r2 r3 r4
       md_count_v md_region_lv idx2 2ul;
     allocate_slab_aux_2_full size_class
-      slab_region md_bm_region md_region md_count r1 r2 r3
-      md_count_v md_region_lv idx1 idx2 idx3;
+      slab_region md_bm_region md_region md_count r1 r2 r3 r4
+      md_count_v md_region_lv idx1 idx2 idx3 idx4;
     return r
   ) else (
     (**) pack_slab_starseq size_class
-      slab_region md_bm_region md_region md_count r1 r2 r3
+      slab_region md_bm_region md_region md_count r1 r2 r3 r4
       md_count_v md_region_lv idx2 1ul;
     assert (Seq.upd (G.reveal md_region_lv) (US.v idx2) 1ul `Seq.equal` md_region_lv);
     (**) starseq_weakening
@@ -689,10 +703,12 @@ let allocate_slab_aux_2
       (SeqUtils.init_u32_refined (U32.v md_count_v))
       (SeqUtils.init_u32_refined (U32.v md_count_v));
     allocate_slab_aux_2_partial size_class
-      slab_region md_bm_region md_region md_count r1 r2 r3
-      md_count_v md_region_lv idx1 idx2 idx3;
+      slab_region md_bm_region md_region md_count r1 r2 r3 r4
+      md_count_v md_region_lv idx1 idx2 idx3 idx4;
     return r
   )
+
+// checkpoint
 
 #push-options "--fuel 0 --ifuel 0"
 let empty_md_is_properly_zeroed
